Games/games/PickUpBricksExtra.lean
@@ -1,0 +1,16 @@
+
+
+
+/-
+Pick-up-bricks, but the first player may take 3 bricks at most once in the game.
+
+Then fst player have win strat: if bricks div by 3, take 3, then play with usual win strat ;
+if bricks not div by 3, play usual win strat.
+
+The point is that this game is not entirely state dependent. Since the first player can play a
+specific move only once, the fst_legal function can not depend only on the current state, but
+requires the history.
+
+Good for illustrating expressivity of my formalism.
+
+-/
